next up: trying to figure out another formulation for transitivity that does mutual induction with typing -- going to start with minimal subset that includes type selections and refinements

src/coq/dot/meta_inversion.v
@@ -1,297 +1,15 @@
 Set Implicit Arguments.
 Require Import List.
 Require Import syntax_binding theory theory_alg.
-Require Import Metatheory LibTactics_sf support meta_regular meta_binding meta_weakening.
+Require Import Metatheory LibTactics_sf support meta_regular meta_binding meta_weakening meta_narrowing.
 Require Import Coq.Program.Equality.
 Require Import Coq.Classes.Equivalence.
 Require Import Coq.Classes.EquivDec.
 Require Import Coq.Logic.Decidable.
 
 
-Lemma path_from_path_eq : forall E p p', path_eq E p p' -> path p /\ path p'.
-Proof. intros. Hint Constructors path. dependent induction H; jauto. Qed.
-
-Lemma path_from_path_safe : forall E p, path_safe E p -> path p.
-Proof. intros. Hint Constructors path. dependent induction H; auto. Qed.
-Hint Resolve path_from_path_safe.
-
-Hint Extern 1 (path ?p) =>
-  match goal with
-  | H: path (sel p ?l) |- _ => inversion H
-  | H: path_eq _ p _ |- _ => apply (proj1 (path_from_path_eq H)); auto
-  | H: path_eq _ _ p |- _ => apply (proj2 (path_from_path_eq H)); auto
-  end.
-
-
-(* E, z : Tz, F on paper is reversed in the mechanisation, since new bindings are prepended*)
-Definition splice_env (E: ctx) z F (s: store) Tz := (F ++ [(z, (Tz, (precise, true)))] ++ E, s).
-
-Instance EqDec_eq_atom `(@EqDec atom eq eq_equivalence) : EqDec_eq atom.
-Proof. trivial. Defined.
-
-Lemma uniq_from_wf_env : forall E s, wf_env (E, s) -> uniq E.
-Proof. 
-intros.
-dependent induction H; eauto.
-Qed.
-Hint Resolve uniq_from_wf_env.
-
-(* internal: specialize hypotheses with satisfiable embedded equalities, drop the (SEEMINGLY) unsatisfiable ones *)
-Ltac sphyps :=
-  repeat match goal with H: ?T |- _ => 
-    match T with
-    | context [?a = _]  => 
-      match type of a with
-        | ?x => try (let h := fresh in lets h: H (@eq_refl x); generalizes h); clear H
-      end
-    | path ?p -> _  =>  (* can't just try to strip any old hypothesis, too wild! *)
-       try (let h := fresh in let Hp := fresh in assert (path p) as Hp by eauto; lets h: H Hp; generalizes h); clear H
-    | _ => generalizes H
-    end
-  end.
-
-(* use this tactic (with care, since it may drop valid hypotheses) to 
-     - instantiate the equalities that arise from dependent induction, 
-     - destruct conjunctions, ... *)
-Ltac simplhyps :=  jauto_set_hyps; intros; sphyps; intros; jauto_set_hyps; intros.
-Ltac simplhyps_except H :=  jauto_set_hyps; intros; generalize H; sphyps; intros; jauto_set_hyps; intros.
-
-(* the resulting quality is precise iff the q' for each member was precise, otherwise subsumed
-  intuitively, collect all the qualities for the individual members, find the minimum, and presto!
-  now, how to convince coq? *)
-Lemma sub_decls_from_exists_sub_decl : forall L E T DS1 DS2,
- (forall z : atom, z `notin` L ->
-    forall (l : label) (d1 d2 : decl),
-    lbl.binds l d2 (DS2 ^ds^ z) ->
-    lbl.binds l d1 (DS1 ^ds^ z) ->
-    exists q', sub_decl (ctx_bind E z T) q' d1 d2)
- -> exists q, 
-   (forall z, z \notin L -> forall_decls (ctx_bind E z T) (DS1 ^ds^ z) (DS2 ^ds^ z) (fun E => fun d1 => fun d2 => sub_decl E q d1 d2)).
-Proof. 
-  intros. pick fresh z for L. specialize (H z Fr).
-  (* try to construct H's other premises, so we can get to the goodies *)
-(*    
-  Lemma forall_decls_nil_1 : forall E q DS,
-   forall_decls E nil DS  (fun (E0 : env) (d1 d2 : decl) => sub_decl E0 q d1 d2).
-  Proof. 
-  Lemma forall_decls_nil_2 : forall E q DS,
-   forall_decls E DS nil (fun (E0 : env) (d1 d2 : decl) => sub_decl E0 q d1 d2).
-  Proof. 
-  Hint Resolve forall_decls_nil_1 forall_decls_nil_2.
-  induction DS1; induction DS2; try solve [simpl in *; eauto | idtac]. 
-
-  destruct a. destruct a0. simpl_env in *.
-  forwards : H ; eauto.*)
-
-Admitted. (* TODO: meh, should be a mere technical Coq hurdle -- obviously true, right? what could possibly go wrong *)
-
-
-Section VarsOk.
-  Hint Unfold ctx_bind.
-  Hint Constructors vars_ok_tp vars_ok_decl vars_ok_tm vars_ok_decls vars_ok_args.
-
-  Let P (e : env) (t : tp)   (v : vars_ok_tp e t)     := forall X bi E s bi' F, e = ((F ++ X ~ bi ++ E), s) -> vars_ok_tp ((F ++ X ~ bi' ++ E), s) t.
-  Let P0 (e : env) (d : decl) (v : vars_ok_decl e d)  := forall X bi E s bi' F, e = ((F ++ X ~ bi ++ E), s) -> vars_ok_decl ((F ++ X ~ bi' ++ E), s) d.
-  Let P1 (e : env) (t : tm)   (v : vars_ok_tm e t)    := forall X bi E s bi' F, e = ((F ++ X ~ bi ++ E), s) -> vars_ok_tm ((F ++ X ~ bi' ++ E), s) t.
-  Let P2 (e : env) (d : decls)(v : vars_ok_decls e d) := forall X bi E s bi' F, e = ((F ++ X ~ bi ++ E), s) -> vars_ok_decls ((F ++ X ~ bi' ++ E), s) d.
-  Let P3 (e : env) (a : args) (v : vars_ok_args e a)  := forall X bi E s bi' F, e = ((F ++ X ~ bi ++ E), s) -> vars_ok_args ((F ++ X ~ bi' ++ E), s) a.
-  Lemma vars_ok_narrowing : 
-   (forall (e : env) (t : tp)   (v : vars_ok_tp e t),   @P  e t v) /\
-   (forall (e : env) (d : decl) (v : vars_ok_decl e d), @P0 e d v) /\
-   (forall (e : env) (t : tm)   (v : vars_ok_tm e t),   @P1 e t v) /\
-   (forall (e : env) (d : decls)(v : vars_ok_decls e d),@P2 e d v) /\
-   (forall (e : env) (a : args) (v : vars_ok_args e a), @P3 e a v).
-  Proof with simpl_env; eauto.
-    apply vars_ok_mutind; intros; unfold P, P0, P1, P2, P3 in *; subst; clear P P0 P1 P2 P3; eauto; intros; subst.
-
-    simplhyps; eapply vars_ok_tp_rfn; eauto; intros x Fr; unfold ctx_bind in *; simpl in *; 
-      eapply H1 with (F0 := ((x, (t, (precise, true))) :: F)); simpl; eauto.
-
-    injsubst H; analyze_binds b...
-    injsubst H; analyze_binds b...
-
-    simplhyps; eapply vars_ok_lam; eauto; intros x Fr; unfold ctx_bind in *; simpl in *; 
-      eapply H1 with (F0 := ((x, (t, (precise, true))) :: F)); simpl; eauto.
-
-    eapply vars_ok_new; eauto; intros x Fr; unfold ctx_bind in *; simpl in *; [
-      eapply H0 with (F0 := ((x, (t, (precise, true))) :: F)) |
-      eapply H1 with (F0 := ((x, (t, (precise, true))) :: F)) ]; simpl; eauto.
-  Qed.
-End VarsOk.
-
-Lemma narrowing_vars_ok_tp : forall X bi E s bi' F T, vars_ok_tp ((F ++ X ~ bi ++ E), s) T -> vars_ok_tp ((F ++ X ~ bi' ++ E), s) T. 
-Proof. intros. destructs vars_ok_narrowing. eapply H0; eauto. Qed.
-
-Lemma narrowing_path_safe : forall F z T q T' q' E s p,
- path_safe (F ++ z ~ (T, (q, true)) ++ E, s) p -> path_safe (F ++ z ~ (T', (q', true)) ++ E, s) p.
-Proof. intros. 
-  Hint Constructors path_safe. 
-  dependent induction H; eauto.  
-   intros. 
-    destruct (x == z). 
-      (* x === z *) destruct e. 
-        analyze_binds H; eapply path_safe_fvar; eauto.
-
-      (* x =/= z *) unfold equiv, complement in *.
-        analyze_binds H; eauto.
-Qed.
-
-Section Q.
-Lemma quality_subsumption : forall E t T q, E |= t ~: T @ precise -> E |= t ~: T @ q.
-Proof.  Hint Resolve sub_tp_refl.
-intros. replace q with (precise & q). eapply typing_sub; eauto. induction q; unfold qconj; simpl; eauto. Qed.
-End Q.
-
-Section NarrowingTyping.
-  Hint Constructors sub_decl sub_qual path_eq wf_env wf_tp wf_decl.
-  Hint Resolve typing_var typing_ref typing_sel typing_peq typing_app typing_lam typing_new expands_rfn expands_and expands_or expands_top expands_bot 
-sub_tp_rfn sub_tp_rfn_elim sub_tp_tpsel_lower sub_tp_tpsel_upper sub_tp_refl sub_tp_top sub_tp_bot sub_tp_fun sub_tp_and_r sub_tp_or_l sub_tp_and_l1 sub_tp_and_l2 sub_tp_or_r1 sub_tp_or_r2. (* typing/expands/subtyping minus transitivity-like rules *)
-  Hint Resolve narrowing_vars_ok_tp narrowing_path_safe.
-
-  Let Ptyp (E: ctx) (s: store) (Sz Tz: tp) (Ez : env) (q: quality) (t: tm) (T: tp) (H: Ez |=  t ~: T  @ q) :=  forall F z,
-    Ez = splice_env E z F s Tz -> path t -> exists q, (splice_env E z F s Sz) |= t ~: T @ q. 
-  Let Pexp (E: ctx) (s: store) (Sz Tz: tp) (Ez : env) (q : quality) (T : tp) (DS : decls) (H: Ez |= T ~< DS @ q) := forall F z,
-    Ez = splice_env E z F s Tz -> exists q, (splice_env E z F s Sz) |= T ~< DS @ q.
-  Let Psub (E: ctx) (s: store) (Sz Tz: tp) (Ez : env) (q : quality) (T1 T2 : tp) (H: Ez |= T1 ~<: T2 @ q) := forall F z,
-    Ez = splice_env E z F s Tz -> exists q, (splice_env E z F s Sz) |= T1 ~<: T2 @ q.
-  Let Psbd (E: ctx) (s: store) (Sz Tz: tp) (Ez : env) (q : quality) (d1 d2 : decl) (H: sub_decl Ez q d1 d2) :=  forall F z ,
-    Ez = splice_env E z F s Tz -> exists q, sub_decl (splice_env E z F s Sz) q d1 d2.
-  Let Ppeq (E: ctx) (s: store) (Sz Tz: tp) (Ez : env) (t1 t2 : tm) (H: path_eq Ez t1 t2) :=  forall F z , 
-    Ez = splice_env E z F s Tz -> path_eq (splice_env E z F s Sz) t1 t2.
-  Let Pwfe (E: ctx) (s: store) (Sz Tz: tp) (Ez : env) (H: wf_env Ez) :=  forall F z , 
-    Ez = splice_env E z F s Tz -> wf_env (splice_env E z F s Sz).
-  Let Pwft (E: ctx) (s: store) (Sz Tz: tp) (Ez : env) (T : tp) (H: wf_tp Ez T) :=  forall F z , 
-    Ez = splice_env E z F s Tz -> wf_tp (splice_env E z F s Sz) T.
-  Let Pwfd (E: ctx) (s: store) (Sz Tz: tp) (Ez : env) (d : decl) (H: wf_decl Ez d) :=  forall F z , 
-    Ez = splice_env E z F s Tz -> wf_decl (splice_env E z F s Sz) d.
-
-
-Lemma sub_narrowing_typing : forall E s Sz Tz qz,
-  (E, s) |= Sz ~<: Tz @ qz ->
- ((forall Ez q t T (H: Ez |= t ~: T @ q), (@Ptyp E s Sz Tz Ez q t T H)) /\ 
-  (forall Ez q T DS (H: Ez |= T ~< DS @ q), (@Pexp E s Sz Tz Ez q T DS H)) /\ 
-  (forall Ez q T T' (H: Ez |= T ~<: T' @ q), (@Psub E s Sz Tz Ez q T T' H))  /\ 
-  (forall (Ez : env) (q : quality) (d d0 : decl) (H : sub_decl Ez q d d0), (@Psbd E s Sz Tz Ez q d d0 H)) /\  
-  (forall (Ez : env) (t t0 : tm) (H : path_eq Ez t t0), (@Ppeq E s Sz Tz Ez t t0 H)) /\  
-  (forall (Ez : env) (H : wf_env Ez), (@Pwfe E s Sz Tz Ez H)) /\
-  (forall (Ez : env) (t : tp) (H : wf_tp Ez t), (@Pwft E s Sz Tz Ez t H)) /\  
-  (forall (Ez : env) (d : decl) (H : wf_decl Ez d), (@Pwfd E s Sz Tz Ez d H))).
-Proof. 
-  introv HSubZ.
-  mutind_typing  (@Ptyp E s Sz Tz) (@Pexp E s Sz Tz) (@Psub E s Sz Tz) (@Psbd E s Sz Tz) (@Ppeq E s Sz Tz) (@Pwfe E s Sz Tz) (@Pwft E s Sz Tz) (@Pwfd E s Sz Tz);  unfold Ptyp, Pexp, Psub, Psbd, Ppeq, Pwfe, Pwft, Pwfd in *; clear Ptyp Pexp Psub Psbd Ppeq Pwfe Pwft Pwfd; unfold splice_env in *; intros; subst;
-    try solve [ auto 
-              | inversion H; subst; symmetry in H1; contradiction (app_cons_not_nil _ (z, (Tz, (precise, true))) F E H1) (* wf_env_nil *)
-              | exists precise; eauto (* sub_tp_refl *)
-(* eauto messes up on the previous two cases, so they must be handled separately -- see below *)
-              | eauto 
-              | injsubst H0; eauto
-              | match goal with H: ?T |- _ =>  match T with
-                 | path ?p  => try solve [inversion H | idtac] end end
-              | simplhyps; eauto
-              | simplhyps; simplhyps; try solve [ eauto
-                  | eexists; eapply typing_sub with (S := S); eauto
-                  | eexists; eapply expands_sub with (U := U); eauto
-                  | eexists; eapply sub_tp_trans with (TMid := TMid); eauto]]. 
-
-  (* typing_var *)
-    injsubst H0.
-    destruct (x == z). 
-      (* x === z *) destruct e. 
-        (* recover that Tz = T from binding in hypothesis b *)
-        analyze_binds_uniq b; eauto; injsubst BindsTacVal.
-
-        (* first construct precise typing for x : Sz *)
-        forwards Hprecise : typing_var (F ++ [(x, (Sz, (precise, true)))] ++ E) s x Sz precise; eauto. 
-          simpl in H. eapply H; eauto.  (* wf_env *)
-
-        eexists; eapply typing_sub; eauto. 
-          eapply weakening_subtyping; eauto; simpl; simpl_alist; fsetdec.
-
-      (* x =/= z *) unfold equiv, complement in *.
-        eexists; eapply typing_var; eauto. 
-          analyze_binds_uniq b; eauto.
-
-  (* sub_tp_rfn *) 
-  simplhyps_except a; simplhyps_except a. rename x into qtp. rename x0 into qx. 
-  
-Lemma narrow_sub_decls_from_narrow_sub_decl_pt1 : forall L DS1 DS2 F z Tz E s T Sz,
- (forall z0 : atom,
-       z0 `notin` L ->
-       forall (l : label) (d1 d2 : decl),
-       lbl.binds l d2 (DS2 ^ds^ z0) ->
-       lbl.binds l d1 (DS1 ^ds^ z0) ->
-       forall (F0 : list (atom * (tp * (quality * bool)))) (z1 : atom),
-       ctx_bind (F ++ [(z, (Tz, (precise, true)))] ++ E, s) z0 T = (F0 ++ [(z1, (Tz, (precise, true)))] ++ E, s) ->
-       exists q,
-       sub_decl (F0 ++ [(z1, (Sz, (precise, true)))] ++ E, s) q d1 d2)
- ->
- (forall z0 : atom,
-       z0 `notin` L ->
-       forall (l : label) (d1 d2 : decl),
-       lbl.binds l d2 (DS2 ^ds^ z0) ->
-       lbl.binds l d1 (DS1 ^ds^ z0) ->
-       exists q,
-       sub_decl (ctx_bind (F ++ [(z, (Sz, (precise, true)))] ++ E, s) z0 T) q d1 d2).
-Proof. intros.
-  forwards : H; eauto; [ 
-    unfold ctx_bind; simpl; f_equal; instantiate (1 := z); instantiate (1 := ((z0, (T, (precise, true))) :: F)); trivial
-    | eapply H3].
-Qed.
- 
-set (@narrow_sub_decls_from_narrow_sub_decl_pt1 L DS1 DS2 F z Tz E s T Sz H2) as Hds0.
-remember ((F ++ [(z, (Sz, (precise, true)))] ++ E, s)) as Eds in Hds0.
-replace ((F ++ [(z, (Sz, (precise, true)))] ++ E, s)) with Eds in *.
-
-
-  destruct (@sub_decls_from_exists_sub_decl L _ _ DS1 DS2 Hds0) as [qds Hds].
-
-Lemma  narrow_sub_decls_from_narrow_sub_decl_pt2 : forall L E T DS1 DS2 q q',
-   (forall z, z \notin L -> forall_decls (ctx_bind E z T) (DS1 ^ds^ z) (DS2 ^ds^ z) (fun E => fun d1 => fun d2 => sub_decl E q d1 d2))
-->
-   (forall z, z \notin L -> forall_decls (ctx_bind E z T) (DS1 ^ds^ z) (DS2 ^ds^ z) (fun E => fun d1 => fun d2 => sub_decl E (q & q') d1 d2)).
-Proof.
-  intros. unfold forall_decls in *; intros. forwards : H; eauto. induction q; induction q'; unfold qconj in *; simpl in *; induction H3; eauto.
-Qed.
-
-  set (@narrow_sub_decls_from_narrow_sub_decl_pt2 L Eds T DS1 DS2 qds (q & (qtp & qx)) Hds) as Hsubds.
-  eexists; eapply sub_tp_rfn; eauto; intros; induction q; induction qds; induction qtp; induction qx; split; forwards [Hdom Hq] : a; auto.
-
-
-  (* sub_tp_tpsel_lower *) (* Ltac just drives me MAD -- why is this case not covered by simplhyps; simplhyps? good luck finding out *)
-    forwards [qtp Htp]: H; eauto. forwards [qx Hx]: H0; auto. eexists; eauto.
-
-  (*  wf_env_cons *)
-  induction F; inverts H0; simpl_env in *; eauto.
-  
-  (* wf_tp_rfn *)
-  eapply wf_rfn; eauto; intros x Fr l d' Hin; unfold ctx_bind in *; simpl in *; 
-    eapply (H0 x Fr l d' Hin ((x, (tp_rfn T DS, (precise, true))) :: F)); simpl; eauto.
-
-(* at some point Coq was sore: "Error: Attempt to save a proof with existential variables still non-instantiated" even though there are no subgoals left because eauto discharges goals while leaving existentials uninstantiated in certain cases
-
-diagnosed using Show Proof.  -- relevant excerpts:
-  (let case := "sub_tp_refl" in
-          fun (E0 : env) (T : tp) (q : quality)
-            (F : list (atom * (tp * (quality * bool)))) 
-            (z : atom) (_ : E0 = (F ++ [(z, (Tz, (precise, true)))] ++ E, s)) =>
-          ex_intro
-            (fun q0 : quality =>
-             (F ++ [(z, (Sz, (precise, true)))] ++ E, s) |= T ~<: T @ q0)
-            ?28778
-            (sub_tp_refl (F ++ [(z, (Sz, (precise, true)))] ++ E, s) T ?28778))
-  (let case := "wf_env_nil" in
-          fun (P : store) (F : list (atom * (tp * (quality * bool))))
-            (z : atom)
-            (H : (nil, P) = (F ++ [(z, (Tz, (precise, true)))] ++ E, s)) =>
-          ?35 E s Sz Tz qz HSubZ P F z H)
-*)
-Qed.
-End NarrowingTyping.
-
-
-
-(* the motivation for the notrans version of subtyping: inversion *)
-Lemma invert_fun_notrans : forall E Sa Sr Ta Tr,
+(* the motivation for the alg version of subtyping: inversion *)
+Lemma invert_fun_alg : forall E Sa Sr Ta Tr,
   E |= tp_fun Sa Sr ~<! tp_fun Ta Tr ->
   E |= Ta ~<! Sa  /\  E |= Sr ~<! Tr.
 Proof.
@@ -299,33 +17,202 @@ intros.
 inverts H; splits; auto using sub_tp_alg_refl.
 Qed.
 
+(* NEEDED BY PRESERVATION (needs soundness and completeness of the algorithmic system + invert_fun_alg)
+Lemma invert_subtyping_fun : 
+   (forall E q T DS, E |= T ~< DS @ q -> forall T1 T2, is_fun T T1 T2 -> DS = nil) /\
+   (forall E q S T, E |= S ~<: T @ q -> forall T1 T2, is_fun S T1 T2 ->
+      (exists T1', exists T2', is_fun T T1' T2' /\ (exists q, E |= T1' ~<: T1 @ q /\ exists q, E |= T2 ~<: T2' @ q))).
 
-
-
-
-
-(*  TODO: add E |== s and E |= ok judgements
 *)
-Lemma sub_tp_notrans_trans_tpsel : forall E q1 q2 p T DS l S U T' DS' S' U' Ta Tb,
+
+Hint Constructors sub_tp_alg sub_decl_alg.
+
+
+
+
+
+Definition exposed E p L S U := exists T DS,  path p /\ E |= p ~:! T /\ E |= T ~<! (tp_rfn tp_top DS) /\ lbl.binds L (decl_tp S U) DS.
+Hint Unfold exposed.
+
+(* strategy for sub_tp_alg_trans_tpsel
+
+(`expose p.L S U` is short for   p : T0 {... L : S'..U' ...} where S = S' ^^ p, U = U' ^^ p)
+
+[case for sub_tp_alg_trans: type selection on the inside]
+
+                 expose p.L S U       expose p.L S' U'
+[sub_tp_tpsel_r]----------------     ----------------[sub_tp_tpsel_l]
+                     S <: p.L          p.L <: U'
+
+NTS: S <: U'
+
+required lemma's, which hopefully do not require transitivity -- BZZZZ they do need it
+
+splice: expose p.L S U -> expose p.L S' U' -> expose p.L S U'
+
+  this should be provable by inverting the typing/subtyping judgements that derive exposure, 
+  cutting each of them in half and splicing them back together to get the required mongrel
+  (if they derive new bounds for L, there must be a sub_decl judgement involved, which is simply 
+  subtyping of the lower and upper bound according to the variance position, thus we can piece together
+  a new sub_decl judgement from the appropriate halves of each one) 
+  
+  --> the problem is you need to induct on these derivations and fuse them together, which requires transitivity
+
+invert_expose: expose p.L S U' -> S <: U' (under suitable side conditions of well-formedness of the context)
+
+
+[case for sub_tp_alg_trans: type selection on the outside -- actually two symmetric cases]
+
+                expose p.L S U
+[sub_tp_tpsel_l]----------------   ----------[??]
+                    p.L <: U         U <: T
+
+invert the sub_tp_alg_rfn_r in expose p.L S U, reconstruct new one by incorporating U <: T
+done
+
+*)
+
+(*
+mutually induct
+need transitivity on types of p (T, T') for path selection case during induction
+*)
+Lemma alg_typing_sub_tp_function_modulo_sub_tp : 
+  forall E p T T', path p -> E |= p ~:! T -> E |= p ~:! T' -> E |= T ~<! T' \/ E |= T' ~<! T.
+  forall E p T DS L D DS' D', path p -> E |= T ~<! (tp_rfn tp_top DS) -> lbl.binds L D DS -> E |= T ~<! (tp_rfn tp_top DS') -> lbl.binds L D' DS'
+  -> sub_decl_alg E (D ^d^ p) (D' ^d^ p) \/ sub_decl_alg E (D' ^d^ p) (D ^d^ p).
+Proof.
+
+
+Lemma splice_exposed : forall E p T T', path p -> E |= p ~:! T -> E |= p ~:! T' -> True.
+Proof.
+  introv Hp Htp Htp'.  skip. skip. skip. skip. skip. skip. skip. skip. skip. skip. skip. skip.  skip. 
+    unfold exposed in Hxpo. inversion Hxpo as [T [DS [Hpath [Htp [Hsub Hbind]]]]].
+    unfold exposed in Hxpo'. inversion Hxpo' as [T' [DS' [_ [Htp' [Hsub' Hbind']]]]]. clear Hxpo Hxpo'.
+    induction p; inverts Hpath; inverts Htp; inverts Htp'. ; dependent induction Hsub; dependent induction Hsub'.
+ induction Hpath; inverts Htp; inverts Htp'; eauto. skip. skip. skip. skip. skip. skip. skip. skip. skip.
+   
+Lemma sub_tp_alg_trans_tpsel : forall E q1 q2 p T DS l S U T' DS' S' U' Ta Tb,
   path_safe E p ->
 
-  E |= p ~:! T ->
+  E |= p ~: T @ q1 ->
   E |= T ~<! tp_rfn tp_top DS ->
   lbl.binds l (decl_tp S U) DS ->
 
-  E |= p ~:! T' -> 
+  E |= p ~: T' @ q2 -> 
   E |= T' ~<! tp_rfn tp_top DS' ->
   lbl.binds l (decl_tp S' U') DS' ->
 
-  E |= S ^tp^ p ~<! U' ^tp^ p.
+  E |= Ta ~<! S ^tp^ p ->
+  E |= U' ^tp^ p ~<! Tb ->
+
+  E |= Ta ~<! Tb.
 Proof. Admitted. (* TODO *)
 
 
+Definition transitivity_on TMid := forall E T T',  E |= T ~<! TMid -> E |= TMid ~<! T' -> E |= T ~<! T'.
+Hint Unfold transitivity_on.
+
+
+
+(* inspired by sub_transitivity from http://www.chargueraud.org/arthur/research/2007/binders/src/Fsub_Soundness.html
+
+  Coq provides "dependent induction" to perform "Induction/inversion principle"; 4.2.1. of
+   http://www.msr-inria.inria.fr/~gares/jar09.pdf explains the latter is needed to perform a proof like this
+*)
+Lemma sub_tp_alg_trans : forall TMid, transitivity_on TMid.
+Proof.
+ introv HSubL HSubR. gen E T T'. gen_eq TMid as TMid' eq. gen TMid' eq. 
+ induction TMid; intros; gen T';
+   induction HSubL; try discriminate; inversions eq; intros; 
+     generalize_eqs_vars HSubR; induction HSubR; simplify_dep_elim; subst; auto; try solve [ 
+       eapply sub_tp_alg_rfn_r; eauto 2; eapply narrow_sub_decls; eauto 2 |
+       eapply sub_tp_alg_and_r; eauto 2 | 
+       eapply sub_tp_alg_and_l1; eapply IHHSubL; eauto 2 |
+       eapply sub_tp_alg_and_l2; eapply IHHSubL; eauto 2 |
+       eapply sub_tp_alg_rfn_l; eapply IHHSubL; eauto 2 |
+       eapply sub_tp_alg_tpsel_l; eauto 3 using sub_tp_alg_rfn_r |
+       eapply sub_tp_alg_or_l; eauto 3 using IHHSubL1, sub_tp_alg_tpsel_l, IHHSubL2 |
+       eapply sub_tp_alg_rfn_r; eauto 3 using IHHSubR1, narrow_sub_decls, sub_tp_alg_rfn_r, IHHSubR2 |
+       eapply sub_tp_alg_fun; eauto 2 using IHTMid1, IHTMid2 |
+       eauto 3]. (* less than 2 minutes*)
+
+(* TODO: the core case... do we need to introduce some kind of sub_tp_alg rule? as in fsub? *)
+rename t into p. rename T into Ta. rename T0 into Tb'. rename T' into Twoele. rename T'0 into T'. rename Twoele into T.
+rename DS0 into DS'. rename S0 into S'. rename U0 into U'. rename q0 into q'. rename q1 into q.
+
+clear IHHSubR1 IHHSubR2 IHHSubL1 IHHSubL2.
+(*
+  H1 : path_safe E p
+  H4 : path p
+
+  H0 : E |= p ~: T @ q
+  HSubL2 : E |= T ~<! tp_rfn tp_top DS
+  H : lbl.binds l (decl_tp S U) DS
+
+  H3 : E |= p ~: T' @ q'
+  HSubR2 : E |= T' ~<! tp_rfn tp_top DS'
+  H2 : lbl.binds l (decl_tp S' U') DS'
+
+  HSubL1 : E |= Ta ~<! S ^tp^ p
+  HSubR1 : E |= U' ^tp^ p ~<! Tb'
+  ============================
+   E |= Ta ~<! Tb
+*)
+
+ eapply sub_tp_alg_trans_tpsel with (T' := T'); eauto.
+Qed.
+
+(*
+sub_tp_alg_or_l, sub_tp_alg_trans_tpsel, sub_tp_alg_trans_rfn_rfn, 
+       try solve [ apply IHHSubR; eauto | 
+                   apply sub_tp_alg_or_l; eauto | 
+                   eauto using rework_sub_decls |
+                   eapply sub_tp_alg_trans_tpsel with (T' := T'); eauto |
+                   eapply sub_tp_alg_trans_rfn_rfn; eauto |
+                   ]. (* 7 min *)
+*)
 
 
 
 
-Hint Constructors sub_tp_notrans sub_decl_notrans.
+Section AlgCompleteness.
+
+    Let P2_ (E : env) (q : quality) (S T : tp) (H: E |= S ~<: T @ q) := E |= S ~<! T.
+    Let P1_ (E : env) (q : quality) (T : tp) (DS : decls) (H: E |= T ~< DS @ q) := E |= T ~<! tp_rfn tp_top DS.
+
+    Let P0_ (E_s: env) (q: quality) (t: tm) (T: tp) (H: E_s |=  t ~: T  @ q) := True.
+    Let P3_ (e : env) (q : quality) (d d0 : decl) (H: sub_decl e q d d0) := True.
+    Let P4_ (e : env) (t t0 : tm) (H: path_eq e t t0) := True.
+    Let P5_ (e : env) (H: wf_env e) := True.
+    Let P6_ (e : env) (t : tp) (H: wf_tp e t) := True.
+    Let P7_ (e : env) (d : decl) (H: wf_decl e d) := True.
+
+  (* only hard case is sub_tp_trans, which is proven above *)
+  Lemma alg_is_complete : (forall E q S T, E |= S ~<: T @ q -> E |= S ~<! T) /\ (forall E q T DS, E |= T ~< DS @ q -> E |= T ~<! tp_rfn tp_top DS).
+  Proof.
+    cut ((forall E q t T (H: E |= t ~: T @ q), (@P0_ E q t T H)) /\ 
+    (forall E q T DS (H: E |= T ~< DS @ q), (@P1_ E q T DS H)) /\ 
+    (forall E q T T' (H: E |= T ~<: T' @ q), (@P2_  E q T T' H))  /\ 
+    (forall (e : env) (q : quality) (d d0 : decl) (H : sub_decl e q d d0), (@P3_ e q d d0 H)) /\  
+    (forall (e : env) (t t0 : tm) (H : path_eq e t t0), (@P4_ e t t0 H)) /\  
+    (forall (e : env) (H : wf_env e), (@P5_ e H)) /\
+    (forall (e : env) (t : tp) (H : wf_tp e t), (@P6_ e t H)) /\  
+    (forall (e : env) (d : decl) (H : wf_decl e d), (@P7_ e d H))); [tauto | 
+      apply (typing_mutind P0_ P1_ P2_ P3_ P4_ P5_ P6_ P7_); unfold P0_, P1_, P2_, P3_, P4_, P5_, P6_, P7_ in *; clear P0_ P1_ P2_ P3_ P4_ P5_ P6_ P7_]; intros; eauto 3. 
+
+    apply sub_tp_alg_trans with (TMid := U); eauto.
+    eapply sub_tp_alg_rfn_r; eauto. 
+    skip. (* TODO: sub_decls_alg_refl *) skip.
+    eapply sub_tp_alg_rfn_r with (DS1 := DS1); eauto 2. 
+    skip. (* TODO: IH for sub_decls (change from True above to something useful) *)
+    apply and_decls_nil_1.
+    apply sub_tp_alg_trans with (TMid := TMid); eauto.
+  Qed.
+
+End AlgCompleteness.
+
+
+
 
 Section Soundness.
   (* TODO: deal with regularity  *)
@@ -362,7 +249,7 @@ Section Soundness.
       skip. (*refl*)
       eapply IHDS'; eauto.
 *)
-6
+
 Lemma sub_decls_sound : forall L E DS1 DS2 T,
   (forall z : atom, z `notin` L -> forall (l : label) (d1 d2 : decl),
    lbl.binds l d2 (DS2 ^ds^ z) -> lbl.binds l d1 (DS1 ^ds^ z) ->
@@ -410,19 +297,20 @@ Qed.
     eapply sub_tp_rfn with (DS1 := DS) (DS2 := DS) (q := subsumed); [
       eauto 3 | eauto 3 | pick fresh z and apply sub_decls_refl | fsetdec | intros; discriminate].
 
-
+(* TODO: switch to full mutual induction that includes typing: also need to prove it sound *)
   Let P (E : env) (T1 T2 : tp) (H : E |= T1 ~<! T2) := (exists q, E |= T1 ~<: T2 @ q) /\ (forall DS, T2 = tp_rfn tp_top DS -> exists q, E |= T1 ~< DS @ q).
-  Let P0 (E : env) (D1 D2 : decl) (H : sub_decl_notrans E D1 D2) := exists q, sub_decl E q D1 D2.
-  Lemma notrans_is_sound : (forall (E : env) (T1 T2 : tp) (H : E |= T1 ~<! T2), @P E T1 T2 H) /\
-              (forall (E : env) (D1 D2 : decl) (H : sub_decl_notrans E D1 D2), @P0 E D1 D2 H). 
-  Proof. unfold P, P0. clear P P0.
-    apply sub_tp_notrans_mutind; first [ (split; 
+  Let P0 (E : env) (D1 D2 : decl) (H : sub_decl_alg E D1 D2) := exists q, sub_decl E q D1 D2.
+  Lemma alg_is_sound : (forall (E : env) (T1 T2 : tp) (H : E |= T1 ~<! T2), @P E T1 T2 H) /\
+              (forall (E : env) (D1 D2 : decl) (H : sub_decl_alg E D1 D2), @P0 E D1 D2 H). 
+  Proof. Admitted. (*unfold P, P0. clear P P0.
+    apply sub_tp_alg_mutind; first [ (split; 
          [ (* subtyping *) simplhyps; try solve [ exists precise; eauto (* to instantiate sub_tp_refl's existential quality *) | eauto 3 | idtac ]
          | (* expansion *) introv HEq; try injsubst HEq; subst; 
-             try destructs IHsub_tp_notrans1; try destructs IHsub_tp_notrans2; try destructs IHsub_tp_notrans; 
+             try destructs IHsub_tp_alg1; try destructs IHsub_tp_alg2; try destructs IHsub_tp_alg; 
              simplhyps; try solve [ discriminate | eauto 2 | eexists; eapply expands_sub; eauto 2 | eexists; intros; eauto 3]]) 
          | (* sub_decl *) intros; exists subsumed; simplhyps; eauto 
-      ];
+      ].
+
       [ eexists; eapply sub_tp_trans with (TMid := tp_sel p L); eauto using sub_tp_trans
       | eexists; eapply expands_sub with (U := tp_sel p L); eauto  using sub_tp_trans
       | eexists; eapply sub_tp_rfn with (L := L) (DS1 := DS1) (DS2 := DS2) (q := subsumed); eauto 3 using expands_sub; intros; discriminate
@@ -431,14 +319,12 @@ Qed.
       | eexists; eapply sub_tp_trans with (TMid := tp_or T1 T2); [eauto 2 | sub_tp_rfn_top DSM]
       | eexists; sub_tp_rfn_top (nil : decls); eauto using expands_sub
       | eexists; eapply expands_sub with (U := tp_rfn tp_top DS); eauto].
-  Qed. (* 5s *)
+  Qed. (* 5s *) *)
 End Soundness.
 (* Show Existentials is your friend when combatting uninstantiated existentials before Coq will let you Qed *)
 
 
 
-Definition transitivity_on TMid := forall E T T',  E |= T ~<! TMid -> E |= TMid ~<! T' -> E |= T ~<! T'.
-Hint Unfold transitivity_on.
 
 Section Narrowing.
   (* specialize hypotheses with satisfiable embedded equalities, drop the unsatisfiable ones *)
@@ -459,19 +345,19 @@ Section Narrowing.
   Let P (E: ctx) (s: store) (Sz Tz: tp) (Ez : env) (S T : tp) (H : Ez |= S ~<! T) := forall F z, 
     Ez = splice_env E z F s Tz -> (splice_env E z F s Sz) |= S ~<! T.
 
-  Let P0 (E: ctx) (s: store) (Sz Tz: tp) (Ez : env) (D1 D2 : decl) (H : sub_decl_notrans Ez D1 D2) := forall F z,
-    Ez = splice_env E z F s Tz -> sub_decl_notrans (splice_env E z F s Sz) D1 D2.
+  Let P0 (E: ctx) (s: store) (Sz Tz: tp) (Ez : env) (D1 D2 : decl) (H : sub_decl_alg Ez D1 D2) := forall F z,
+    Ez = splice_env E z F s Tz -> sub_decl_alg (splice_env E z F s Sz) D1 D2.
 
 Lemma sub_narrowing_aux : forall s E Sz Tz,
 (*  transitivity_on Tz -> *)
   (E, s) |= Sz ~<! Tz ->
     (forall (Ez : env) (T1 T2 : tp) (H : Ez |= T1 ~<! T2), @P E s Sz Tz Ez T1 T2 H) /\
-    (forall (Ez : env) (D1 D2 : decl) (H : sub_decl_notrans Ez D1 D2), @P0 E s Sz Tz Ez D1 D2 H).
+    (forall (Ez : env) (D1 D2 : decl) (H : sub_decl_alg Ez D1 D2), @P0 E s Sz Tz Ez D1 D2 H).
 Proof. 
   unfold P, P0. clear P P0. introv (*HTrans*) HSubZ. 
-  destruct (proj1 ((proj1 notrans_is_sound) _ _ _ HSubZ)) as [qsz Hsz].
+  destruct (proj1 ((proj1 alg_is_sound) _ _ _ HSubZ)) as [qsz Hsz].
 
-  apply sub_tp_notrans_mutind; intros; subst; simplhyps; eauto 4.
+  apply sub_tp_alg_mutind; intros; subst; simplhyps; eauto 4.
 
 (*Hint Extern 1 (splice_env ?E ?z ?F ?s ?Sz |= ?p ~: ?T @ ?q) =>
   match goal with
@@ -484,9 +370,9 @@ Proof.
   
   Hint Resolve narrowing_vars_ok_tp narrowing_path_safe.
   forwards [qn Hn] : (proj1 (sub_narrowing_typing Hsz)); eauto 2.
-  eapply sub_tp_notrans_tpsel_r; unfold splice_env in *; eauto. 
+  eapply sub_tp_alg_tpsel_r; unfold splice_env in *; eauto. 
 
-  eapply sub_tp_notrans_rfn_r; eauto.   
+  eapply sub_tp_alg_rfn_r; eauto.   
     intros zd Frd.  specialize (H1 zd Frd). 
     unfold forall_decls, ctx_bind, splice_env in *. simpl in *. simpl_env in *.
   intros. forwards : H1; eauto. simpl; f_equal. instantiate (1 := z). instantiate (1 :=  (zd, (T, (precise, true))) :: F). trivial. simpl_env in *. trivial.
@@ -498,9 +384,9 @@ Lemma narrow_sub_decls: forall L E S T DS1 DS2,
 (*  transitivity_on T ->*)
   E |=  S ~<! T ->
   (forall z : atom, z `notin` L ->
-     forall_decls (ctx_bind E z T) (DS1 ^ds^ z) (DS2 ^ds^ z) sub_decl_notrans) -> 
+     forall_decls (ctx_bind E z T) (DS1 ^ds^ z) (DS2 ^ds^ z) sub_decl_alg) -> 
   (forall z : atom, z `notin` L ->
-     forall_decls (ctx_bind E z S) (DS1 ^ds^ z) (DS2 ^ds^ z) sub_decl_notrans).
+     forall_decls (ctx_bind E z S) (DS1 ^ds^ z) (DS2 ^ds^ z) sub_decl_alg).
 Proof. 
   unfold forall_decls. intros. forwards : H0; eauto. unfold ctx_bind in *. destruct E. simpl in *. 
   forwards : (proj2 (sub_narrowing_aux H)); eauto. unfold splice_env; simpl; f_equal. instantiate (1 := z). instantiate (1 := nil). auto. eapply H5.
@@ -509,154 +395,6 @@ Qed.
 Hint Resolve narrow_sub_decls.
 
 
-(* strategy for sub_tp_notrans_trans_tpsel
-
-(`expose p.L S U` is short for   p : T0 {... L : S'..U' ...} where S = S' ^^ p, U = U' ^^ p)
-
-[case for sub_tp_notrans_trans: type selection on the inside]
-
-                 expose p.L S U       expose p.L S' U'
-[sub_tp_tpsel_r]----------------     ----------------[sub_tp_tpsel_l]
-                     S <: p.L          p.L <: U'
-
-NTS: S <: U'
-
-required lemma's, which hopefully do not require transitivity
-
-splice: expose p.L S U -> expose p.L S' U' -> expose p.L S U'
-
-  this should be provable by inverting the typing/subtyping judgements that derive exposure, 
-  cutting each of them in half and splicing them back together to get the required mongrel
-  (if they derive new bounds for L, there must be a sub_decl judgement involved, which is simply 
-  subtyping of the lower and upper bound according to the variance position, thus we can piece together
-  a new sub_decl judgement from the appropriate halves of each one) 
-
-invert_expose: expose p.L S U' -> S <: U' (under suitable side conditions of well-formedness of the context)
-
-
-[case for sub_tp_notrans_trans: type selection on the outside -- actually two symmetric cases]
-
-                expose p.L S U
-[sub_tp_tpsel_l]----------------   ----------[??]
-                    p.L <: U         U <: T
-
-invert the sub_tp_notrans_rfn_r in expose p.L S U, reconstruct new one by incorporating U <: T
-done
-
-*)
-Lemma sub_tp_notrans_trans_tpsel : forall E q1 q2 p T DS l S U T' DS' S' U' Ta Tb,
-  path_safe E p ->
-
-  E |= p ~: T @ q1 ->
-  E |= T ~<! tp_rfn tp_top DS ->
-  lbl.binds l (decl_tp S U) DS ->
-
-  E |= p ~: T' @ q2 -> 
-  E |= T' ~<! tp_rfn tp_top DS' ->
-  lbl.binds l (decl_tp S' U') DS' ->
-
-  E |= Ta ~<! S ^tp^ p ->
-  E |= U' ^tp^ p ~<! Tb ->
-
-  E |= Ta ~<! Tb.
-Proof. Admitted. (* TODO *)
-
-(* inspired by sub_transitivity from http://www.chargueraud.org/arthur/research/2007/binders/src/Fsub_Soundness.html
-
-  Coq provides "dependent induction" to perform "Induction/inversion principle"; 4.2.1. of
-   http://www.msr-inria.inria.fr/~gares/jar09.pdf explains the latter is needed to perform a proof like this
-*)
-Lemma sub_tp_notrans_trans : forall TMid, transitivity_on TMid.
-Proof.
- introv HSubL HSubR. gen E T T'. gen_eq TMid as TMid' eq. gen TMid' eq. 
- induction TMid; intros; gen T';
-   induction HSubL; try discriminate; inversions eq; intros; 
-     generalize_eqs_vars HSubR; induction HSubR; simplify_dep_elim; subst; auto; try solve [ 
-       eapply sub_tp_notrans_rfn_r; eauto 2; eapply narrow_sub_decls; eauto 2 |
-       eapply sub_tp_notrans_and_r; eauto 2 | 
-       eapply sub_tp_notrans_and_l1; eapply IHHSubL; eauto 2 |
-       eapply sub_tp_notrans_and_l2; eapply IHHSubL; eauto 2 |
-       eapply sub_tp_notrans_rfn_l; eapply IHHSubL; eauto 2 |
-       eapply sub_tp_notrans_tpsel_l; eauto 3 using sub_tp_notrans_rfn_r |
-       eapply sub_tp_notrans_or_l; eauto 3 using IHHSubL1, sub_tp_notrans_tpsel_l, IHHSubL2 |
-       eapply sub_tp_notrans_rfn_r; eauto 3 using IHHSubR1, narrow_sub_decls, sub_tp_notrans_rfn_r, IHHSubR2 |
-       eapply sub_tp_notrans_fun; eauto 2 using IHTMid1, IHTMid2 |
-       eauto 3]. (* less than 2 minutes*)
-
-(* TODO: the core case... do we need to introduce some kind of sub_tp_notrans rule? as in fsub? *)
-rename t into p. rename T into Ta. rename T0 into Tb'. rename T' into Twoele. rename T'0 into T'. rename Twoele into T.
-rename DS0 into DS'. rename S0 into S'. rename U0 into U'. rename q0 into q'. rename q1 into q.
-
-clear IHHSubR1 IHHSubR2 IHHSubL1 IHHSubL2.
-(*
-  H1 : path_safe E p
-  H4 : path p
-
-  H0 : E |= p ~: T @ q
-  HSubL2 : E |= T ~<! tp_rfn tp_top DS
-  H : lbl.binds l (decl_tp S U) DS
-
-  H3 : E |= p ~: T' @ q'
-  HSubR2 : E |= T' ~<! tp_rfn tp_top DS'
-  H2 : lbl.binds l (decl_tp S' U') DS'
-
-  HSubL1 : E |= Ta ~<! S ^tp^ p
-  HSubR1 : E |= U' ^tp^ p ~<! Tb'
-  ============================
-   E |= Ta ~<! Tb
-*)
-
- eapply sub_tp_notrans_trans_tpsel with (T' := T'); eauto.
-Qed.
-
-(*
-sub_tp_notrans_or_l, sub_tp_notrans_trans_tpsel, sub_tp_notrans_trans_rfn_rfn, 
-       try solve [ apply IHHSubR; eauto | 
-                   apply sub_tp_notrans_or_l; eauto | 
-                   eauto using rework_sub_decls |
-                   eapply sub_tp_notrans_trans_tpsel with (T' := T'); eauto |
-                   eapply sub_tp_notrans_trans_rfn_rfn; eauto |
-                   ]. (* 7 min *)
-*)
-
-
-
-
-Section Completeness.
-
-    Let P2_ (E : env) (q : quality) (S T : tp) (H: E |= S ~<: T @ q) := E |= S ~<! T.
-    Let P1_ (E : env) (q : quality) (T : tp) (DS : decls) (H: E |= T ~< DS @ q) := E |= T ~<! tp_rfn tp_top DS.
-
-    Let P0_ (E_s: env) (q: quality) (t: tm) (T: tp) (H: E_s |=  t ~: T  @ q) := True.
-    Let P3_ (e : env) (q : quality) (d d0 : decl) (H: sub_decl e q d d0) := True.
-    Let P4_ (e : env) (t t0 : tm) (H: path_eq e t t0) := True.
-    Let P5_ (e : env) (H: wf_env e) := True.
-    Let P6_ (e : env) (t : tp) (H: wf_tp e t) := True.
-    Let P7_ (e : env) (d : decl) (H: wf_decl e d) := True.
-
-  (* only hard case is sub_tp_trans, which is proven above *)
-  Lemma notrans_is_complete : (forall E q S T, E |= S ~<: T @ q -> E |= S ~<! T) /\ (forall E q T DS, E |= T ~< DS @ q -> E |= T ~<! tp_rfn tp_top DS).
-  Proof.
-    cut ((forall E q t T (H: E |= t ~: T @ q), (@P0_ E q t T H)) /\ 
-    (forall E q T DS (H: E |= T ~< DS @ q), (@P1_ E q T DS H)) /\ 
-    (forall E q T T' (H: E |= T ~<: T' @ q), (@P2_  E q T T' H))  /\ 
-    (forall (e : env) (q : quality) (d d0 : decl) (H : sub_decl e q d d0), (@P3_ e q d d0 H)) /\  
-    (forall (e : env) (t t0 : tm) (H : path_eq e t t0), (@P4_ e t t0 H)) /\  
-    (forall (e : env) (H : wf_env e), (@P5_ e H)) /\
-    (forall (e : env) (t : tp) (H : wf_tp e t), (@P6_ e t H)) /\  
-    (forall (e : env) (d : decl) (H : wf_decl e d), (@P7_ e d H))); [tauto | 
-      apply (typing_mutind P0_ P1_ P2_ P3_ P4_ P5_ P6_ P7_); unfold P0_, P1_, P2_, P3_, P4_, P5_, P6_, P7_ in *; clear P0_ P1_ P2_ P3_ P4_ P5_ P6_ P7_]; intros; eauto 3. 
-
-    apply sub_tp_notrans_trans with (TMid := U); eauto.
-    eapply sub_tp_notrans_rfn_r; eauto. 
-    skip. (* TODO: sub_decls_notrans_refl *) skip.
-    eapply sub_tp_notrans_rfn_r with (DS1 := DS1); eauto 2. 
-    skip. (* TODO: IH for sub_decls (change from True above to something useful) *)
-    apply and_decls_nil_1.
-    apply sub_tp_notrans_trans with (TMid := TMid); eauto.
-  Qed.
-
-End NoTransSoundComplete.
 
 
 (* more convenient interface to above *)
