src/coq/dot/meta_mini_trans.v
@@ -1,0 +1,136 @@
+Set Implicit Arguments.
+Require Import List.
+Require Import syntax_binding theory_mini.
+Require Import Metatheory LibTactics_sf support.
+
+
+Definition exposed E p L S U := exists T DS,  path p /\ E |= p ~:% T /\ E |= T ~<% (tp_rfn tp_top DS) /\ lbl.binds L (decl_tp S U) DS.
+Hint Unfold exposed.
+
+(* strategy for sub_tp_alg_trans_tpsel
+
+(`expose p.L S U` is short for   p : T0 {... L : S'..U' ...} where S = S' ^^ p, U = U' ^^ p)
+
+[case for sub_tp_alg_trans: type selection on the inside]
+
+                 expose p.L S U       expose p.L S' U'
+[sub_tp_tpsel_r]----------------     ----------------[sub_tp_tpsel_l]
+                     S <: p.L          p.L <: U'
+
+NTS: S <: U'
+
+required lemma's, which hopefully do not require transitivity -- BZZZZ they do need it
+
+splice: expose p.L S U -> expose p.L S' U' -> expose p.L S U'
+
+  this should be provable by inverting the typing/subtyping judgements that derive exposure, 
+  cutting each of them in half and splicing them back together to get the required mongrel
+  (if they derive new bounds for L, there must be a sub_decl judgement involved, which is simply 
+  subtyping of the lower and upper bound according to the variance position, thus we can piece together
+  a new sub_decl judgement from the appropriate halves of each one) 
+  
+  --> the problem is you need to induct on these derivations and fuse them together, which requires transitivity
+
+invert_expose: expose p.L S U' -> S <: U' (under suitable side conditions of well-formedness of the context)
+
+
+[case for sub_tp_alg_trans: type selection on the outside -- actually two symmetric cases]
+
+                expose p.L S U
+[sub_tp_tpsel_l]----------------   ----------[??]
+                    p.L <: U         U <: T
+
+invert the sub_tp_alg_rfn_r in expose p.L S U, reconstruct new one by incorporating U <: T
+done
+
+*)
+
+(*
+mutually induct
+need transitivity on types of p (T, T') for path selection case during induction
+*)
+Lemma alg_typing_sub_tp_function_modulo_sub_tp : 
+  forall E p T T', path p -> E |= p ~:% T -> E |= p ~:% T' -> E |= T ~<% T' \/ E |= T' ~<% T.
+  forall E p T DS L D DS' D', path p -> E |= T ~<% (tp_rfn tp_top DS) -> lbl.binds L D DS -> E |= T ~<% (tp_rfn tp_top DS') -> lbl.binds L D' DS'
+  -> sub_decl_alg E (D ^d^ p) (D' ^d^ p) \/ sub_decl_alg E (D' ^d^ p) (D ^d^ p).
+Proof.
+
+
+Lemma splice_exposed : forall E p T T', path p -> E |= p ~:% T -> E |= p ~:% T' -> True.
+Proof.
+  introv Hp Htp Htp'.  skip. skip. skip. skip. skip. skip. skip. skip. skip. skip. skip. skip.  skip. 
+    unfold exposed in Hxpo. inversion Hxpo as [T [DS [Hpath [Htp [Hsub Hbind]]]]].
+    unfold exposed in Hxpo'. inversion Hxpo' as [T' [DS' [_ [Htp' [Hsub' Hbind']]]]]. clear Hxpo Hxpo'.
+    induction p; inverts Hpath; inverts Htp; inverts Htp'. ; dependent induction Hsub; dependent induction Hsub'.
+ induction Hpath; inverts Htp; inverts Htp'; eauto. skip. skip. skip. skip. skip. skip. skip. skip. skip.
+   
+Lemma sub_tp_alg_trans_tpsel : forall E q1 q2 p T DS l S U T' DS' S' U' Ta Tb,
+  path_safe E p ->
+
+  E |= p ~: T @ q1 ->
+  E |= T ~<% tp_rfn tp_top DS ->
+  lbl.binds l (decl_tp S U) DS ->
+
+  E |= p ~: T' @ q2 -> 
+  E |= T' ~<% tp_rfn tp_top DS' ->
+  lbl.binds l (decl_tp S' U') DS' ->
+
+  E |= Ta ~<% S ^tp^ p ->
+  E |= U' ^tp^ p ~<% Tb ->
+
+  E |= Ta ~<% Tb.
+Proof. Admitted. (* TODO *)
+
+
+Definition transitivity_on TMid := forall E T T',  E |= T ~<% TMid -> E |= TMid ~<% T' -> E |= T ~<% T'.
+Hint Unfold transitivity_on.
+
+
+
+(* inspired by sub_transitivity from http://www.chargueraud.org/arthur/research/2007/binders/src/Fsub_Soundness.html
+
+  Coq provides "dependent induction" to perform "Induction/inversion principle"; 4.2.1. of
+   http://www.msr-inria.inria.fr/~gares/jar09.pdf explains the latter is needed to perform a proof like this
+*)
+Lemma sub_tp_alg_trans : forall TMid, transitivity_on TMid.
+Proof.
+ introv HSubL HSubR. gen E T T'. gen_eq TMid as TMid' eq. gen TMid' eq. 
+ induction TMid; intros; gen T';
+   induction HSubL; try discriminate; inversions eq; intros; 
+     generalize_eqs_vars HSubR; induction HSubR; simplify_dep_elim; subst; auto; try solve [ 
+       eapply sub_tp_alg_rfn_r; eauto 2; eapply narrow_sub_decls; eauto 2 |
+       eapply sub_tp_alg_and_r; eauto 2 | 
+       eapply sub_tp_alg_and_l1; eapply IHHSubL; eauto 2 |
+       eapply sub_tp_alg_and_l2; eapply IHHSubL; eauto 2 |
+       eapply sub_tp_alg_rfn_l; eapply IHHSubL; eauto 2 |
+       eapply sub_tp_alg_tpsel_l; eauto 3 using sub_tp_alg_rfn_r |
+       eapply sub_tp_alg_or_l; eauto 3 using IHHSubL1, sub_tp_alg_tpsel_l, IHHSubL2 |
+       eapply sub_tp_alg_rfn_r; eauto 3 using IHHSubR1, narrow_sub_decls, sub_tp_alg_rfn_r, IHHSubR2 |
+       eapply sub_tp_alg_fun; eauto 2 using IHTMid1, IHTMid2 |
+       eauto 3]. (* less than 2 minutes*)
+
+(* TODO: the core case... do we need to introduce some kind of sub_tp_alg rule? as in fsub? *)
+rename t into p. rename T into Ta. rename T0 into Tb'. rename T' into Twoele. rename T'0 into T'. rename Twoele into T.
+rename DS0 into DS'. rename S0 into S'. rename U0 into U'. rename q0 into q'. rename q1 into q.
+
+clear IHHSubR1 IHHSubR2 IHHSubL1 IHHSubL2.
+(*
+  H1 : path_safe E p
+  H4 : path p
+
+  H0 : E |= p ~: T @ q
+  HSubL2 : E |= T ~<% tp_rfn tp_top DS
+  H : lbl.binds l (decl_tp S U) DS
+
+  H3 : E |= p ~: T' @ q'
+  HSubR2 : E |= T' ~<% tp_rfn tp_top DS'
+  H2 : lbl.binds l (decl_tp S' U') DS'
+
+  HSubL1 : E |= Ta ~<% S ^tp^ p
+  HSubR1 : E |= U' ^tp^ p ~<% Tb'
+  ============================
+   E |= Ta ~<% Tb
+*)
+
+ eapply sub_tp_alg_trans_tpsel with (T' := T'); eauto.
+Qed.
